
$$\begin{align}
    A = \{X = \min \{X , Y\} \}
\end{align}$$
(1) $Y\geq X$ 时

$$\begin{align}
    \min \{X , Y\} = X 
\end{align}$$

(2) $Y<X$

$$\begin{align}
    \min \{X , Y\} = Y 
\end{align}$$

所以事件 $A$ 等价于 $B = \{Y \geq X \}$ 计算

$$\begin{align}
    P(A) &= P(B) \\
    &= P\{Y \geq X\} \\
    &=\int^{+\infty}_{0} dx \int^{+\infty}_xe^{-x} 2e^{-2y}dy \\
    &=\int^{+\infty}_{0} e^{-x} -e^{-2y}|^{+\infty}_xdx \\
    &=\int^{+\infty}_0e^{-3x} dx\\
    &= \frac{1}{3}
\end{align}$$

考点:


$$\begin{align}
    U = \min \{X , Y\} \rightarrow U \leq X , U \leq Y \\
    U = \max \{X , Y\} \rightarrow U \geq X , U \geq Y
\end{align}$$

---



设 $a_n = \displaystyle \int^{\frac{\pi}{2}}_0 \frac{\sin 2nx }{\sin x} dx$ .
(1) 求 $\displaystyle \lim_{n\rightarrow \infty} (a_n - a_{n-1})$
(2)求 $\displaystyle \lim_{n\rightarrow \infty} a_n$
(1)解:
因为 $a_n = \displaystyle \int^{\frac{\pi}{2}}_0 \frac{\sin 2nx }{\sin x} dx$

$$\begin{align}
    a_n -a_{n-1} &= \int^{\frac{\pi}{2}}_0 \frac{\sin 2nx  - \sin (2n - 2)x}{\sin x} dx \\
    &=\int^{\frac{\pi}{2}}_0 \frac{2\sin x \cos (\frac{2n + 2n -2}{2}) x}{\sin x} dx \\
    &=\int^{\frac{\pi}{2}}_0 \frac{2\sin x \cos  (2n - 1)x}{\sin x} dx \\
    &=\int^{\frac{\pi}{2}}_0  2\cos  (2n - 1)x dx \\
    &=\frac{2}{2n - 1} \sin(2n - 1)x |^{\frac{\pi}{2}}_0 \\
    &=\frac{2}{2n - 1}\sin(n\pi - \frac{\pi}{2}) \\
    &= \begin{cases}
        \frac{-2}{2n - 1} , n= 2k \\
        \frac{2}{2n - 1} , n=2k+1
    \end{cases} \\
    &= \frac{2(-1)^{n-1}}{2n-1}
\end{align}$$

注意到 $a_1 = \displaystyle \int^{\frac{\pi}{2}}_0 \frac{\sin 2x }{\sin x} dx = \int^{\frac{\pi}{2}}_0 \frac{2\sin x \cos x }{\sin x} dx = 2\sin x|^\frac{\pi}{2}_0 = 2$ ,满足 $a_n$ 通项,则

$$\begin{align}
    a_n  - a_{n-1} = \frac{2(-1)^{n-1}}{2n-1}\rightarrow \lim_{n\rightarrow \infty} (a_n - a_{n-1}) = 0
\end{align}$$


(2)因为

$$\begin{align}
    a_2 - a_1 &= \frac{(-1)2}{3} \\
    a_3 - a_2 &= \frac{2}{5} \\
    &\vdots \\
    a_n  - a_{n-1} &= \frac{2(-1)^{n-1}}{2n-1}
\end{align}$$

求和得到

$$\begin{align}
    a_{n} - a_1 &= 2\sum_{k=1}^{n}  \frac{(-1)^{k}}{2k+1} \rightarrow a_n = 2\sum_{k=0}^{n}  \frac{(-1)^{k}}{2k+1}
\end{align}$$

因为

$$\begin{align}
    \arctan x &= \sum_{n=1}^{\infty} \frac{(-1)^{n-1}x^n}{2n - 1} \\
    &=\sum_{n=0}^{\infty} \frac{(-1)^{n}x^{n+1}}{2n + 1}
\end{align}$$

得到 $\arctan 1 = \displaystyle \sum_{n=0}^{\infty} \frac{(-1)^{n}}{2n + 1}$ ,所以

$$\begin{align}
    \lim_{n\rightarrow \infty} a_n &= 2\sum_{k=0}^{\infty}  \frac{(-1)^{n}}{2n+1}\\
    &=2\arctan 1\\
    &=\frac{\pi}{2}
\end{align}$$


---
解
$$\begin{align}
    F(s)&= e^{-2s}\frac{1}{(s + 1)(s^2 + 2s + 5)} \\
    &=e^{-2s}[\frac{1}{4} \frac{1}{1+s} + \frac{-1}{4}\frac{s + 1}{(s^2 + 2s + 5)}] \\
    &=e^{-2s}[\frac{1}{4} \frac{1}{1+s} + \frac{-1}{4}\frac{s + 1}{(s+1)^2 + 4}]
\end{align}$$

令
$$\begin{align}
    h(t) = [\frac{1}{4}e^{-t} - \frac{1}{4}e^{-t}\cos 2t]\varepsilon(t)
\end{align}$$

则
$$\begin{align}
    f(t) = h(t - 2)
\end{align}$$




$$\begin{align}
    H(s) &= \sum_{k=0}^\infty a^k e^{-ksT} \\
\end{align}$$


其中 $s = \sigma + jw$ ,注意到如果这个式子收敛,则
$$\begin{align}
    \lim_{n\rightarrow \infty} \frac{|a^{n+ 1}e^{-(n + 1)Ts}|}{|a^{n}e^{-nTs}|} &=\lim_{n\rightarrow \infty} |ae^{-Ts}| \\
    &=\lim_{n\rightarrow \infty} |ae^{-T\sigma}e^{-jwT}| \\
    &=ae^{-T\sigma}<1
\end{align}$$

得到收敛域 $\sigma > \frac{1}{T} \ln a$,那么此时上式有
$$\begin{align}
    \sum_{k=0}^\infty a^k e^{-ksT} &= \sum_{k=0}^\infty (ae^{-sT})^k\\
    &=\frac{1}{1 - ae^{-sT}}
\end{align}$$



解:
$$\begin{align}
    y(t - t_0) = \int^{3t - 3t_0}_{-\infty} f(\tau) d\tau 
\end{align}$$

又
$$\begin{align}
    T\{f(t - t_0)\} &=\int^{3t}_{-\infty} f(\tau - t_0) d\tau \\
    &= \int^{3t - t_0}_{-\infty} f(\xi) d\xi  \not ={y(t - t_0)}
\end{align}$$

所以他是时变的.