### 解
解:

$$\begin{align}
    x^TAx &= x_1^2 + 2x_2^2 - 4x_3^2 + 2x_1x_2 - 2 x_2 x_3 \\ 
    &= (x_1^2 + 2x_1x_2)+ (2x_2^2- 2 x_2 x_3) - 4x_3^2 \\
    &= (x_1 + x_2)^2 + x_2^2 - 2x_2x_3 - 4x_3^2 \\
    &=(x_1 + x_2)^2 + (x_2 - x_3)^2 - 5x_3^2
\end{align}$$


令

$$\begin{align}
    \begin{cases}
        y_1 = x_1 + x_2 \\
        y_2 = x_2 - x_3 \\
        y_3 = x_3
    \end{cases} \rightarrow \begin{cases}
        x_1 = y_1 - y_2 - y_3 \\ 
        x_2 = y_2 + y_3 \\
        x_3 = y_3
    \end{cases}
\end{align}$$

则有:

$$\begin{align}
    \begin{bmatrix}
        x_1 \\ x_2 \\ x_3
    \end{bmatrix} = \begin{bmatrix}
        1 & -1 & -1 \\
        0 & 1 & 1\\
        0 & 0 & 1
    \end{bmatrix}\begin{bmatrix}
        y_1 \\ y_2 \\ y_3
    \end{bmatrix}
\end{align}$$

写为

$$\begin{align}
    x = Cy
\end{align}$$

通过等价变换为

$$\begin{align}
    x^TAx &= y^TC^TACx \\
    &= y^T \Lambda x
\end{align}$$

故矩阵 $C$ 为:

$$\begin{align}
    C = \begin{bmatrix}
        1 & -1 & -1 \\
        0 & 1 & 1\\
        0 & 0 & 1
    \end{bmatrix}
\end{align}$$


<<<<<<< HEAD
=======




已知对于三角波函数为

$$\begin{align}
    \Delta_{\tau}(t) =\begin{cases}
        1 - \frac{|t|}{\tau} , |t| \leq \tau \\
        0,else
    \end{cases}
\end{align}$$

它的傅里叶变换为 $F[\Delta_{\tau}(t)] = \tau Sa^2(\frac{w\tau}{2})$,则

$$\begin{align}
    F(jw) &= \frac{\sin^2 3w}{w^2}\cos w\\
    &=9\frac{\sin^2 3w}{(3w)^2} \cos w \\
    &=9\frac{\sin^2 3w}{(3w)^2}[\frac{1}{2}e^{jw} + \frac{1}{2}e^{-jw}] \\
    &=\frac{9}{2}\frac{\sin^2 3w}{(3w)^2}[e^{jw} + e^{-jw}] \\
    &=\frac{9}{12}6Sa^2(\frac{6w}{2})[e^{jw} + e^{-jw}] \\
    &=\frac{3}{4}(6Sa^2(\frac{6w}{2}))[e^{jw} + e^{-jw}]
\end{align}$$

得到原信号为 $\frac{3}{4}[\Delta_{6}(t+1)+\Delta_{6}(t-1)]$


>>>>>>> 182497d (new)
