### 1.非初始松弛状态
#### 1.1 第一种
假设 $y[n]$ 的零输入响应有初始状态 $y[-1],y[-2],\cdots$ ,则
$$\begin{align}
    \sum_{n=0}^\infty y[n]z^{-n} = Y(z)
\end{align}$$

考虑
$$\begin{align}
    \sum_{n=0}^\infty y[n - 1]z^{-n} &= \sum_{n=-1}^\infty y[n]z^{-(n+1)} \\
    &=y[-1] + \sum_{n=0}^\infty y[n]z^{-(n+1)} \\
    &=y[-1] + z^{-1}\sum_{n=0}^\infty y[n]z^{-n} \\
    &=y[-1] + z^{-1}Y(z)
\end{align}$$


既有 $$\begin{align}
    Z\{y[n-1]\} &=z^{-1}Y(z) + y[-1] \\
    &= z^{-1}Z\{y[n]\} + y[0-1] 
\end{align}$$ 

,递推有
$$\begin{align}
    Z\{y[n-2]\} &= Z\{y[(n-1) - 1]\} \\
    &= z^{-1}Z\{y[n-1]\} + y[(0-1)-1] \\
    &=z^{-1}(z^{-1}Y(z) + y[-1]) + y[-2] \\
    &=z^{-2}Y(z) + z^{-1}y[-1] + y[-2]
\end{align}$$

#### 1.2 第二种
假设 $y[n]$ 的零输入响应有状态 $y[0],y[1],y[2]$ ,则

$$\begin{align}
    \sum_{n=0}^\infty y[n]z^{-n} = Y(z)
\end{align}$$

考虑
$$\begin{align}
    \sum_{n=0}^\infty y[n + 1]z^{-n} &=  \sum_{n=1}^\infty y[n]z^{-(n - 1)} \\
    &=\sum_{n=0}^\infty y[n]z^{-(n - 1)} - zy[0] \\
    &=y[1] + z\sum_{n=0}^\infty y[n]z^{-n} - zy[0] \\
    &=zY(z)- zy[0]
\end{align}$$


同理递推有
$$\begin{align}
    Z\{y[(n+1) + 1]\} &= \sum_{n=0}^\infty y[n + 2]z^{-n} \\
    &=\sum_{n=2}^\infty y[n]z^{-(n - 2)} \\
    &=\sum_{n=0}^\infty y[n]z^{-(n - 2)} - z^2y[0] - zy[1] \\
    &=z^2Y(z) - z^2y[0] - zy[1]
\end{align}$$