### 微分算子
令

$$\begin{align}
    \frac{d}{dt} = p \\
    \int^{t}_{-\infty} dt = \frac{1}{p}
\end{align}$$

那么对于微分方程:

$$\begin{align}
    \sum_{i = 0}^n a_iy^{(i)}(t) = \sum_{i = 0}^m b_if^{(i)}(t) ,a_n = 1
\end{align}$$

将 $f(t) = \delta(t)$ 

$$\begin{align}
    h(t) = \frac{\sum_{i = 0}^n b_ip^i}{\sum_{i = 0}^n a_ip^i} \delta(t)
\end{align}$$

令

$$\begin{align}
    H(p) = \frac{\sum_{i = 0}^n b_ip^i}{\sum_{i = 0}^n a_ip^i}
\end{align}$$

##### 1.单根

$$\begin{align}
    H(p) &= \frac{\sum_{i = 0}^n b_ip^i}{\prod_{i=1}^{n}(p - p_i)} \\
    &= \sum^n_{i=1} \frac{C_i}{p - p_i}
\end{align}$$

返回到 (4) 式中有:

$$\begin{align}
    h_i(t) &=\frac{C_i}{p - p_i}\delta(t) \\
    h'_i(t) - p_ih_i(t) &= C_i\delta(t) \rightarrow h_i(t) = C_i e^{p_i t}
\end{align}$$

通过线性有:

$$\begin{align}
    h(t) = \sum_{i = 1}^nC_i e^{p_i t}
\end{align}$$

##### 2.重根
对于:

$$\begin{align}
    h(t) = \frac{C}{(p - p_0)^n} \delta(t) = \frac{C}{(n - 1)!}t^{n-1}e^{p_0t} u(t)
\end{align}$$

例如对于:

$$\begin{align}
    H(p) &= \frac{p^2 + p + 1}{(p + 1)^3} + 1 \\
    &= \frac{2}{p + 1} + \frac{-1}{(p+1)^2} + \frac{1}{(p + 1)^3} + 1
\end{align}$$

得到:

$$\begin{align}
    h(t) &= [2e^{-t} - te^{-t} + \frac{1}{2!}t^2e^{-t} + \delta(t)] \epsilon(t) \\
    &=[2e^{-t} - te^{-t} + \frac{1}{2}t^2e^{-t} + \delta(t)] \epsilon(t)
\end{align}$$

##### 3.共轭复根

$$\begin{align}
    h(t) = \frac{p + \alpha}{(p + \alpha)^2 + \omega^2} \delta(t) = e^{-\alpha t}\cos(\omega t)  \epsilon(t)
\end{align}$$



$$\begin{align}
    h(t) = \frac{\omega}{(p + \alpha)^2 + \omega^2} \delta(t) = e^{-\alpha t}\sin(\omega t)  \epsilon(t)
\end{align}$$

例题:

$$\begin{align}
    H(p)&= \frac{2p + 3}{p^2 + 2p + 2} \\
    &= \frac{2p + 3 }{(p + 1)^2 + 1} \\
    &= 2\frac{p + 1}{(p + 1)^2 + 1} +\frac{1 }{(p + 1)^2 + 1}
\end{align}$$

得到:

$$\begin{align}
    h(t) = [2e^{-t}\cos(t) + e^{-t}\sin(t)]\epsilon(t)
\end{align}$$

总结:与拉普拉斯变换有异曲同工之妙.