### 系统全响应

$$\begin{align}
    y[k] = y_{ZSR}[k] + y_{ZIR}[k]
\end{align}$$

### 1.零输入响应
即齐次解,在已知初始条件下的齐次解, $y_{ZIR}[0],y_{ZIR}[1],\cdots , y_{ZIR}[n-1]$

$$\begin{align}
    \sum_{i = 0}^n a_iy[k+i] = 0 ,a_n = 1
\end{align}$$

### 2.零状态响应
先利用迭代法求得初始条件 $y_{ZSR}[0],y_{ZSR}[1],\cdots , y_{ZSR}[n-1]$ ,再求其解:

$$\begin{align}
    \sum_{i = 0}^n a_iy[k+i] = \sum_{i = 0}^m b_if[k+i] ,a_n = 1
\end{align}$$

求初始状态时,以方程

$$\begin{align}
    \sum_{i = 0}^n a_iy[k+i] = 0 ,a_n = 1
\end{align}$$

取 $k=-n,-n+1,\cdots,1$ ,因为 $y_{ZSR}[k]=0,k\leq -1$,以此分别求得 $y[0],y[1],\cdots y[n-1]$ ,解方程系数即可.

#### 3.例题

