### 系统模型
令:

$$\begin{align}
    Ef[n] = f[n+1] \\
    E^{-1}f[n] = f[n-1]
\end{align}$$

从而系统模型

$$\begin{align}
    \sum_{i = 0}^n a_iy[k+i] = \sum_{i = 0}^m b_if[k+i] ,a_n = 1
\end{align}$$

变为:

$$\begin{align}
    [\sum_{i = 0}^n a_iE^{i}]y[k] = [\sum_{j = 0}^m b_jE^{j}]f[k] ,a_n = 1
\end{align}$$

则有:

$$\begin{align}
    y[k] = \frac{\sum_{j = 0}^m b_jE^{j}}{\sum_{i = 0}^n a_iE^{i}}f[k]
\end{align}$$

令 $f[k] = \delta[k]$ ,则有:

$$\begin{align}
    h[k] = \frac{\sum_{j = 0}^m b_jE^{j}}{\sum_{i = 0}^n a_iE^{i}}\delta[k]
\end{align}$$

令:

$$\begin{align}
    H(E) = \frac{\sum_{j = 0}^m b_jE^{j}}{\sum_{i = 0}^n a_iE^{i}}
\end{align}$$
##### 1.单根

$$\begin{align}
    H(E) &= \frac{\sum_{j = 0}^m b_jE^{j}}{\prod_{i=1}^{n}(E - \gamma_i)} \\
    &= \sum^n_{i=1} \frac{C_i}{E - \gamma_i}
\end{align}$$

则有:

$$\begin{align}
    h_i[k] = \frac{C_i}{E - \gamma_i}\delta[k]
\end{align}$$

其解为:

$$\begin{align}
    k_i[k] = C_i\gamma_i^{k-1}\epsilon[k-1]
\end{align}$$

此外有:

$$\begin{align}
    x[k] &= \frac{CE}{E - \gamma}\delta[k] \\ 
    &= C\delta[k] + \frac{C\gamma}{E - \gamma}\delta[k] \\
    &= C\delta[k] +C\gamma\gamma^{k-1}\epsilon[k-1] \\
    &= C\gamma^k\epsilon[k]
\end{align}$$

有这个以后我们可以:

$$\begin{align}
    \frac{H(E)}{E} &= \frac{\sum_{j = 0}^m b_jE^{j}}{E\prod_{i=1}^{n}(E - \gamma_i)} \\
    &= \sum^n_{i=1} \frac{C_i}{E - \gamma_i}  + \frac{C}{E} 
\end{align}$$

得到:

$$\begin{align}
    H(E) = C + \sum^n_{i=1} \frac{C_iE}{E - \gamma_i}  
\end{align}$$

最后有:

$$\begin{align}
    h[k] = C\delta[k] + \sum_{i=1}^{n}C_i\gamma^k\epsilon[k]
\end{align}$$

##### 2.多重根
对于

$$\begin{align}
    H'(E) &= \frac{H(E)}{E} = \frac{N(E)}{(E - \gamma)^r} \\
    &= \sum_{i=1}^r \frac{C_i}{(E - \gamma)^i}
\end{align}$$

得到:

$$\begin{align}
    H_q(E) = \frac{C_qE}{(E - q)^q}
\end{align}$$

它对应的解为:

$$\begin{align}
    h_q[k] = \frac{C_q}{(q - 1)!} \frac{k!}{(k-q+1)!}\gamma^{k-q+1}\epsilon[k]
\end{align}$$

##### 3.共轭复根
比较难,一般不会出.

