#### 已知 $f_{X|Y}(x|y),f_{Y|X}(y|x)$,求 $f_X(x),f_Y(y)$
因为

$$\begin{align}
    f_{X|Y}(x|y)&= \frac{f_{X,Y}(x,y)}{f_{X}(x)} \\
    f_{Y|X}(y|x)&=\frac{f_{X,Y}(x,y)}{f_{Y}(y)}
\end{align}$$

故

$$\begin{align}
    \frac{f_{X|Y}(x|y)}{f_{Y|X}(y|x)} = \frac{f_X(x)}{f_Y(y)}
\end{align}$$

将其分割,获得概率密度函数.

设二维正态分布 $(X,Y)$ 的概率密度函数为 $f_{X,Y}(x,y)$ ,已知条件概率分布为 $f_{X|Y}(x|y) = \sqrt{\frac{2}{3\pi}}e^{-\frac{2}{3}(x - \frac{y}{2})^2},f_{Y|X}(y|x) = \sqrt{\frac{2}{3\pi}}e^{-\frac{2}{3}(y - \frac{x}{2})^2}$ ,求 $f_{X,Y}(x,y)$.
解:

$$\begin{align}
    \frac{f_{X|Y}(x|y)}{f_{Y|X}(y|x)} = \frac{f_X(x)}{f_Y(y)}
\end{align}$$

我们得到:

$$\begin{align}
    \frac{f_{X|Y}(x|y)}{f_{Y|X}(y|x)} &= e^{-\frac{2}{3}(x^2 - xy + \frac{y^2}{4})+\frac{2}{3}(y^2 - xy + \frac{x^2}{4})} \\
    &=\exp\{-\frac{2}{3} (\frac{3}{4}x^2 - \frac{3}{4}y^2)\}\\
    &=\exp\{-\frac{1}{2}x^2 + \frac{1}{2}y^2\} \\
    &= e^{-\frac{1}{2}x^2 + \frac{1}{2}y^2} \\
    &= \frac{e^{-\frac{1}{2}x^2}}{e^{-\frac{1}{2}y^2}}
\end{align}$$

得到:

$$\begin{align}
    f_X(x) = Ce^{-\frac{1}{2}x^2} \\
    f_Y(y) = Ce^{-\frac{1}{2}y^2}
\end{align}$$

利归一性有:

$$\begin{align}
    \int^{+\infty}_{-\infty} Ce^{-\frac{1}{2}y^2}dy = 1  \rightarrow C = \frac{1}{\sqrt{2\pi}}
\end{align}$$

又:

$$\begin{align}
    f_{X,Y}(x,y) &= f_Y(y)f_{X|Y}(x|y) \\
    &= \frac{1}{\sqrt{2\pi}}e^{-\frac{1}{2}y^2}\sqrt{\frac{2}{3\pi}}e^{-\frac{2}{3}(x - \frac{y}{2})^2}\\
\end{align}$$