### 一.实函数
对于一个时域实函数 $f(t)$ 它可以分为:

$$\begin{align}
    f(t) = \frac{f(t) + f(-t)}{2} + \frac{f(t) - f(-t)}{2}
\end{align}$$

令:

$$\begin{align}
    f_e(t) = \frac{f(t) + f(-t)}{2}  \rightarrow f_e(t) = f_e(-t)\\
    f_o(t) = \frac{f(t) - f(-t)}{2}\rightarrow f_o(t) = -f_o(-t)
\end{align}$$

### 二.复函数
对于一个时域实函数 $f(t)$ 它可以分为:

$$\begin{align}
    f(t) = f_r(t) + jf_i(t) \rightarrow f^{*}(t) = f_r(t) - jf_i(t) 
\end{align}$$

可以得到:

$$\begin{align}
    f_r(t) =\frac{f(t) + f^{*}(t)}{2} \\
    f_i(t) =\frac{f(t) - f^{*}(t)}{2j}  
\end{align}$$


他可以写为:

$$\begin{align}
    f(t) = \frac{f(t) + f^{*}(-t)}{2}  + \frac{f(t) - f^{*}(t)}{2}
\end{align}$$

此时令:

$$\begin{align}
    f_e(t) = \frac{f(t) + f^{*}(-t)}{2} \rightarrow f_e(t) = f_e^{*}(-t)\\
    f_o(t) = \frac{f(t) - f^{*}(t)}{2}\rightarrow f_o(t) = -f_o^{*}(-t)
\end{align}$$

这写分量在分析傅里叶变换的时候非常有用.
